vale/code/arch/x64/interop/new/Vale.AsLowStar.Test.fst
@@ -1,0 +1,28 @@
+module Vale.AsLowStar.Test
+open Interop.Base
+module ME = X64.Memory
+module IA = Interop.Assumptions
+module V = X64.Vale.Decls
+module IX64 = Interop.X64
+module VSig = Vale.AsLowStar.ValeSig
+module LSig = Vale.AsLowStar.LowStarSig
+module W = Vale.AsLowStar.Wrapper
+
+[@__reduce__] unfold
+let t = TD_Buffer ME.TUInt64
+
+[@__reduce__] unfold
+let dom : (x:list td {List.length x == 2}) =
+  let y = [t;t] in
+  assert_norm (List.length y = 2);
+  y
+
+assume val pre : VSig.vale_pre dom
+assume val post : VSig.vale_post dom
+assume val n : nat
+assume val v: VSig.vale_sig pre post
+assume val c: V.va_code
+
+[@__reduce__]
+let call_c_t = IX64.as_lowstar_sig_t_weak c dom [] _ _ (W.mk_prediction c dom [] n (v c IA.win))
+let call_c : call_c_t = IX64.wrap_weak c dom (W.mk_prediction c dom [] n (v c IA.win))
